src/lowparse/LowParse.Low.VLData.Aux.fsti
@@ -3,13 +3,13 @@ include LowParse.Spec.VLData
 include LowParse.Low.Base
 
 inline_for_extraction
-val parse32_bounded_integer_1 : unit -> Tot (parser32 (parse_bounded_integer 1))
+val parse32_bounded_integer_1 : unit -> Tot (parser32_weak (parse_bounded_integer 1))
 
 inline_for_extraction
-val parse32_bounded_integer_2 : unit -> Tot (parser32 (parse_bounded_integer 2))
+val parse32_bounded_integer_2 : unit -> Tot (parser32_weak (parse_bounded_integer 2))
 
 inline_for_extraction
-val parse32_bounded_integer_3 : unit -> Tot (parser32 (parse_bounded_integer 3))
+val parse32_bounded_integer_3 : unit -> Tot (parser32_weak (parse_bounded_integer 3))
 
 inline_for_extraction
-val parse32_bounded_integer_4 : unit -> Tot (parser32 (parse_bounded_integer 4))
+val parse32_bounded_integer_4 : unit -> Tot (parser32_weak (parse_bounded_integer 4))
